[Checkpoint] Finish implementing Layer 1

src/Common/HoareLogic.v
@@ -5,58 +5,60 @@ Set Implicit Arguments.
 Module Type Layer.
   Parameter oracle : Type.
   Parameter data : Type.
+  Parameter aux_state : Type.
+  Definition state := (aux_state * disk data)%type.
   Parameter prog : Type -> Type.
-  Parameter exec: forall T, oracle -> disk data -> prog T -> @Result (disk data) T -> Prop.
-  Parameter oracle_ok : forall T, prog T -> oracle -> disk data -> Prop.
+  Parameter exec: forall T, oracle -> state -> prog T -> @Result state T -> Prop.
+  Parameter oracle_ok : forall T, prog T -> oracle -> state -> Prop.
 End Layer.
+
+Instance addr_eq_dec: EqDec addr := addr_dec.
 
 Module HoareLogic (l: Layer).
   Import l.
 (** ** Hoare logic *)
-Definition precond := oracle -> @pred addr addr_dec data.
-Definition postcond {T: Type} := T -> @pred addr addr_dec data.
-Definition crashcond := @pred addr addr_dec data.
-Definition augpostcond {T: Type} := oracle -> disk data -> T -> @pred addr addr_dec data.
-Definition augcrashcond := oracle -> disk data -> @pred addr addr_dec data.
+Definition precond := oracle -> aux_state -> @pred addr addr_dec data.
+Definition postcond {T: Type} := T -> aux_state -> @pred addr addr_dec data.
+Definition crashcond := aux_state -> @pred addr addr_dec data.
+Definition augpostcond {T: Type} := oracle -> aux_state -> disk data -> T -> @pred addr addr_dec data.
+Definition augcrashcond := oracle -> aux_state -> disk data -> @pred addr addr_dec data.
 
 Definition hoare_triple {T: Type} (pre: precond) (p: prog T) (post: @postcond T) (crash: crashcond) (augpost: augpostcond) (augcrash: augcrashcond):=
-  fun o d =>
-    pre o d ->
+  fun o d xs =>
+    pre o xs d ->
     (exists ret,
-        exec o d p ret /\
+        exec o (xs, d) p ret /\
         ((exists d' r,
              ret = Finished d' r
-             /\ post r d' /\ augpost o d r d') \/
+             /\ post r (fst d') (snd d') /\ augpost o xs d r (snd d')) \/
          (exists d',
-             ret = Crashed d' /\ crash d' /\ augcrash o d d')))%type.
-
-
+             ret = Crashed d' /\ crash (fst d') (snd d') /\ augcrash o xs d (snd d'))))%type.
   
 Notation
-  "<< o , d >> pre p << r >> post crash" :=
+  "<< o , d , xs >> pre p << r , xsr >> post crash" :=
   (forall F, hoare_triple
-          (fun o d => (F * pre * [[ oracle_ok p o d ]]) d)%pred
+          (fun o xs d => (F * pre * [[ oracle_ok p o (xs, d) ]]) d)%pred
           p%pred
-          (fun r => F * post)%pred
-          (F * crash)%pred
+          (fun r xsr => F * post)%pred
+          (fun xsr => F * crash)%pred
+          (fun _ _ _ _ => any)
           (fun _ _ _ => any)
-          (fun _ _ => any)
-          o d)      
-    (at level 10, o at next level, d at next level, pre at next level, p at next level, r at next level, post at next level, crash at next level,
-     format "'[v' '[  ' '<<' o ','  d '>>' '//' '[' pre ']' '//' '[' p ']' ']' '//' '[  ' '<<' r '>>' '//' '[' post ']' '//' '[' crash ']' ']' ']'").
+          o d xs)      
+    (at level 10, o at next level, d at next level, xs at next level, xsr at next level, pre at next level, p at next level, r at next level, post at next level, crash at next level,
+     format "'[v' '[  ' '<<' o ','  d ','  xs '>>' '//' '[' pre ']' '//' '[' p ']' ']' '//' '[  ' '<<' r ','  xsr '>>' '//' '[' post ']' '//' '[' crash ']' ']' ']'").
 
 Notation
-  "<< o , d >> pre p << r >> post crash augpost augcrash" :=
+  "<< o , d , xs >> pre p << r , xsr >> post crash augpost augcrash" :=
   (forall F, hoare_triple
-          (fun o d => (F * pre * [[ oracle_ok p o d ]]) d)%pred
+          (fun o xs d => (F * pre * [[ oracle_ok p o (xs, d) ]]) d)%pred
           p%pred
-          (fun r => F * post)%pred
-          (F * crash)%pred
-          (fun o d r => F * augpost)%pred
-          (fun o d => F * augcrash)%pred
-          o d)      
-    (at level 10, o at next level, d at next level, pre at next level, p at next level, r at next level, post at next level, crash at next level, augpost at next level, augcrash at next level,
-     format "'[v' '[  ' '<<' o ','  d '>>' '//' '[' pre ']' '//' '[' p ']' ']' '//' '[  ' '<<' r '>>' '//' '[' post ']' '//' '[' crash ']' '//' '[' augpost ']' '//' '[' augcrash ']' ']' ']'").
+          (fun r xsr => F * post)%pred
+          (fun xsr => F * crash)%pred
+          (fun o xs d r  => F * augpost)%pred
+          (fun o xs d => F * augcrash)%pred
+          o d xs)      
+    (at level 10, o at next level, d at next level, xs at next level, xsr at next level, pre at next level, p at next level, r at next level, post at next level, crash at next level, augpost at next level, augcrash at next level,
+     format "'[v' '[  ' '<<' o ','  d ','  xs '>>' '//' '[' pre ']' '//' '[' p ']' ']' '//' '[  ' '<<' r ','  xsr '>>' '//' '[' post ']' '//' '[' crash ']' '//' '[' augpost ']' '//' '[' augcrash ']' ']' ']'").
 
 (*
 Notation
@@ -71,24 +73,24 @@ Notation
 *)
 
 Theorem remember_oracle_ok :
-  forall T (p: prog T) o d pre post crash ap ac,
-    (oracle_ok p o d ->
-  << o, d >>
-   pre
+  forall T (p: prog T) o d a pre post crash (ap: augpostcond) ac,
+ (oracle_ok p o (a, d) ->
+  << o, d, a >>
+   (pre o a)
    p
-  << r >>
-   (post r)
-   crash
-   (ap o d r)
-   (ac o d)) ->
-  << o, d >>
-   pre
+  << r, ar >>
+   (post r ar)
+   (crash ar)
+   (ap o a d r)
+   (ac o a d)) ->
+  << o, d, a >>
+   (pre o a)
    p
-  << r >>
-   (post r)
-   crash
-   (ap o d r)
-   (ac o d).
+  << r, ar >>
+   (post r ar)
+   (crash ar)
+   (ap o a d r)
+   (ac o a d).
 Proof.
   unfold hoare_triple; intros.
   eapply H; eauto.
@@ -97,20 +99,20 @@ Qed.
 
 
 Theorem crash_weaken:
-  forall T (p: prog T) pre post crash1 crash2 o d,
-  << o, d >>
-   pre
+  forall T (p: prog T) pre post crash1 crash2 o d a,
+  << o, d, a >>
+   (pre a)
    p
-  << r >>
-   (post r)
-   crash1 ->
-  (crash1 =p=> crash2) ->
-  << o, d >>
-     pre
+  << r, ar >>
+   (post r ar)
+   (crash1 ar) ->
+  (forall ar, crash1 ar =p=> crash2 ar) ->
+  << o, d, a >>
+     (pre a)
      p
-  << r >>
-     (post r)
-     crash2.
+  << r, ar >>
+     (post r ar)
+     (crash2 ar).
 Proof.
   unfold hoare_triple; intros.
   edestruct H; eauto.
@@ -123,20 +125,20 @@ Qed.
 
 
 Theorem post_weaken:
-  forall T (p: prog T) pre post1 post2 crash o d,
-  << o, d >>
-   pre
+  forall T (p: prog T) pre post1 post2 crash o d a,
+  << o, d, a >>
+   (pre a)
    p
-  << r >>
-   (post1 r)
-   crash  ->
-  (forall r, post1 r =p=> post2 r) ->
-  << o, d >>
-     pre
+  << r, ar >>
+   (post1 r ar)
+   (crash ar)  ->
+  (forall r ar, post1 r ar =p=> post2 r ar) ->
+  << o, d, a >>
+     (pre a)
      p
-  << r >>
-     (post2 r)
-     crash.
+  << r, ar >>
+     (post2 r ar)
+     (crash ar).
 Proof.
   unfold hoare_triple; intros.
   edestruct H; eauto.
@@ -148,20 +150,20 @@ Proof.
 Qed.
 
 Theorem pre_strengthen:
-  forall T (p: prog T) pre1 pre2 post crash o d,
-  << o, d >>
-   pre1
+  forall T (p: prog T) pre1 pre2 post crash o d a,
+  << o, d, a >>
+   (pre1 a)
    p
-  << r >>
-   (post r)
-   crash ->
-  (pre2 =p=> pre1) ->
-  << o, d >>
-     pre2
+  << r, ar >>
+   (post r ar)
+   (crash ar) ->
+  (pre2 a =p=> pre1 a) ->
+  << o, d, a >>
+     (pre2 a)
      p
-  << r >>
-     (post r)
-     crash.
+  << r, ar >>
+     (post r ar)
+     (crash ar).
 Proof.
   unfold hoare_triple; intros.
   edestruct H; eauto.
@@ -169,24 +171,24 @@ Proof.
 Qed.
 
 Theorem pre_strengthen_aug:
-  forall T (p: prog T) pre1 pre2 post crash ap ac o d,
-  << o, d >>
-   pre1
+  forall T (p: prog T) pre1 pre2 post crash ap ac o d a,
+  << o, d, a >>
+   (pre1 a)
    p
-  << r >>
-   (post r)
-   crash
-   (ap o d r)
-   (ac o d) ->
-  (pre2 =p=> pre1) ->
-  << o, d >>
-     pre2
+  << r, ar >>
+   (post r ar)
+   (crash ar)
+   (ap o a d r)
+   (ac o a d) ->
+  (pre2 a =p=> pre1 a ) ->
+  << o, d, a >>
+     (pre2 a)
      p
-  << r >>
-     (post r)
-     crash
-     (ap o d r)
-     (ac o d).
+  << r, ar >>
+     (post r ar)
+     (crash ar)
+     (ap o a d r)
+     (ac o a d).
 Proof.
   unfold hoare_triple; intros.
   edestruct H; eauto.
@@ -195,19 +197,19 @@ Qed.
 
 
 Theorem add_frame:
-  forall T (p: prog T) pre post crash F o d,
-  << o, d >>
-   pre
+  forall T (p: prog T) pre post crash F o d a,
+  << o, d, a >>
+   (pre a)
    p
-  << r >>
-   (post r)
-   crash  ->
-  << o, d >>
-     (F * pre)
+  << r, ar >>
+   (post r ar)
+   (crash ar)  ->
+  << o, d, a >>
+     (F * pre a)
      p
-  << r >>
-     (F * post r)
-     (F * crash).
+  << r, ar >>
+     (F * post r ar)
+     (F * crash ar).
 Proof.
   unfold hoare_triple; intros.
   edestruct H; eauto.
@@ -221,20 +223,20 @@ Proof.
 Qed.
 
 Theorem extract_exists:
-  forall T V (p: prog T) pre post crash o d,
+  forall T V (p: prog T) pre post crash o d a,
     (forall (v:V),
-  << o, d >>
-   (pre v)
+  << o, d, a >>
+   (pre a v)
    p
-  << r >>
-   (post r)
-   crash) ->
-  << o, d >>
-     (exists v, pre v)
+  << r, ar >>
+   (post r ar)
+   (crash ar)) ->
+  << o, d, a >>
+     (exists v, pre a v)
      p
-  << r >>
-     (post r)
-     crash.
+  << r, ar >>
+     (post r ar)
+     (crash ar).
 Proof.
   unfold hoare_triple; intros.
   destruct_lifts.
@@ -243,24 +245,24 @@ Proof.
 Qed.
 
 Theorem extract_exists_aug:
-  forall T V (p: prog T) pre post crash ap ac o d,
+  forall T V (p: prog T) pre post crash ap ac o d a,
     (forall (v:V),
-  << o, d >>
-   (pre v)
+  << o, d, a >>
+   (pre a v)
    p
-  << r >>
-   (post r)
-   crash
-   (ap o d r)
-   (ac o d)) ->
-  << o, d >>
-     (exists v, pre v)
+  << r, ar >>
+   (post r ar)
+   (crash ar)
+   (ap o a d r)
+   (ac o a d)) ->
+  << o, d, a >>
+     (exists v, pre a v)
      p
-  << r >>
-     (post r)
-     crash
-     (ap o d r)
-     (ac o d).
+  << r, ar >>
+     (post r ar)
+     (crash ar)
+     (ap o a d r)
+     (ac o a d).
 Proof.
   unfold hoare_triple; intros.
   destruct_lifts.
@@ -269,31 +271,31 @@ Proof.
 Qed.
 
 Theorem remove_augcons:
-  forall T (p: prog T) pre post crash (augpost: augpostcond) (augcrash: augcrashcond) o d,
-  << o, d >>
-   pre
+  forall T (p: prog T) pre post crash (augpost: augpostcond) (augcrash: augcrashcond) o d a,
+  << o, d, a >>
+   (pre a)
    p
-  << r >>
-   (post r)
-   crash ->
+  << r, ar >>
+   (post r ar)
+   (crash ar) ->
   (forall F d' r,
-      (F * pre)%pred d ->
-      exec o d p (Finished d' r) ->
-      (F * post r)%pred d' ->
-      (F * augpost o d r)%pred d') ->
+      (F * pre a)%pred d ->
+      exec o (a, d) p (Finished d' r) ->
+      (F * post r (fst d'))%pred (snd d') ->
+      (F * augpost o a d r)%pred (snd d')) ->
   (forall F d',
-      (F * pre)%pred d ->
-      exec o d p (Crashed d') ->
-      (F * crash)%pred d' ->
-      (F * augcrash o d)%pred d') ->
-  << o, d >>
-     pre
+      (F * pre a)%pred d ->
+      exec o (a, d) p (Crashed d') ->
+      (F * crash (fst d'))%pred (snd d') ->
+      (F * augcrash o a d)%pred (snd d')) ->
+  << o, d, a >>
+     (pre a)
      p
-  << r >>
-     (post r)
-     crash
-     (augpost o d r)
-     (augcrash o d).
+  << r, ar >>
+     (post r ar)
+     (crash ar)
+     (augpost o a d r)
+     (augcrash o a d).
 Proof.
   unfold hoare_triple; intros.
   edestruct H; eauto; cleanup.
