src/Layer1/Facts.v
@@ -1,7 +1,7 @@
 Require Import Primitives Simulation Layer1.Definitions ProgAuto.
 Import ListNotations.
 
-Lemma exec_crash_in:
+Lemma layer1_exec_crash_in:
   forall T (p: prog T) o d d',
     exec o d p (Crashed d') ->
     In Crash o.
@@ -12,113 +12,81 @@ Proof.
   apply in_app_iff; eauto.
 Qed.
 
-Lemma exec_finished_deterministic:
-  forall T (p: prog T) o1 o2 st st1 st2 r1 r2,
-    exec o1 st p (Finished st1 r1)->
-    exec o2 st p (Finished st2 r2) ->
-    st1 = st2 /\ r1 = r2 /\ o1 = o2.
+Lemma layer1_exec_finished_deterministic:
+  forall T (p: prog T) o1 o2 o3 o4 s s1 s2 r1 r2,
+      exec o1 s p (Finished s1 r1) ->
+      exec o2 s p (Finished s2 r2) ->
+      o1 ++ o3 = o2 ++ o4 ->
+      o1 = o2 /\ s1 = s2 /\ r1 = r2.
 Proof.
-    unfold state; induction p; simpl; intros;
-  invert_exec; cleanup;
-    invert_exec; cleanup;
-      cleanup; eauto.
-    apply encrypt_ext in H5; cleanup;
-    intuition eauto.
-    specialize IHp with (1:=H0)(2:=H1); eauto; cleanup.
-    specialize H with (1:=H2)(2:=H3); cleanup.
-    repeat rewrite app_length; eauto.
+  induction p; simpl; intros;
+    repeat (invert_exec; simpl in *; cleanup);
+    simpl; eauto; try solve [intuition].
+  repeat rewrite <- app_assoc in H2.
+  specialize IHp with (1:= H0)(2:= H1)(3:=H2); cleanup.
+  apply app_inv_head in H2.
+  specialize H with (1:= H4)(2:= H3)(3:=H2); cleanup; eauto.
 Qed.
 
-Lemma exec_finished_oracle_app:
-  forall T (p: prog T) o1 o2 st st1 r1 ret,
-    exec o1 st p (Finished st1 r1)->
-    exec (o1++o2) st p ret ->
-    o2 = [] /\ ret = Finished st1 r1.
+Lemma layer1_finished_not_crashed_oracle_app:
+  forall T (p: prog T) o1 o2 s s1 s2 r1,
+    exec o1 s p (Finished s1 r1) ->
+    ~exec (o1++o2) s p (Crashed s2).
 Proof.
-  unfold state; induction p; simpl; intros;
-    try solve [
-          invert_exec; cleanup;
-          invert_exec; cleanup; 
-          [ match goal with
-            | [H: [_] = [_] ++ _ |- _] =>
-              rewrite app_nil_end in H at 1;
-              apply app_inv_head in H; eauto
-            end|
-            repeat rewrite <- app_cons_nil in *;
-            inversion H1; congruence] ].
-
-  invert_exec; cleanup;
-          invert_exec; cleanup; 
-          [ match goal with
-            | [H: [_] = [_] ++ _ |- _] =>
-              rewrite app_nil_end in H at 1;
-              apply app_inv_head in H; eauto
-            end|
-            repeat rewrite <- app_cons_nil in *;
-            inversion H1; congruence].
-  apply encrypt_ext in H6; cleanup;
-    intuition eauto.
-  
-  invert_exec; cleanup;
-    invert_exec; cleanup.
-    -
-      eapply exec_finished_deterministic in H0; eauto; cleanup.
-      eapply exec_finished_deterministic in H4; eauto; cleanup.
-      rewrite <- app_assoc in H3.
-      apply app_inv_head in H3; cleanup; eauto.
-      setoid_rewrite <- app_nil_r in H3 at 4.
-      apply app_inv_head in H3; cleanup; eauto.
-    -
-      split_ors.
-      +
-        rewrite <- app_assoc in H1; eauto.
-        edestruct IHp; eauto; inversion H4.
-      +
-        eapply exec_finished_deterministic in H0; eauto; cleanup.
-        rewrite <- app_assoc in H4.
-        apply app_inv_head in H4; cleanup; eauto.
+  unfold not; induction p; simpl; intros;
+    repeat (invert_exec; simpl in *; cleanup); simpl; eauto.
+  split_ors; cleanup.
+  -
+    rewrite <- app_assoc in H1; eauto.
+  -
+    rewrite <- app_assoc in H4; eauto.
+    eapply layer1_exec_finished_deterministic in H0; eauto; cleanup; eauto.
+    apply app_inv_head in H4; cleanup; eauto.
 Qed.
 
-Lemma deterministic_prog:
-  forall T (p: prog T) o st ret1 ret2,
-    exec o st p ret1 ->
-    exec o st p ret2 ->
-    ret1 = ret2.
+Lemma layer1_exec_deterministic:
+  forall T (p: prog T) o s r1 r2,
+      exec o s p r1 ->
+      exec o s p r2 ->
+      r1 = r2.
 Proof.
-  unfold state; induction p; simpl; intros;
-  invert_exec; cleanup;
-    invert_exec; cleanup;
-      try solve [intuition eauto].
-  - apply encrypt_ext in H6; cleanup; intuition eauto.
+  induction p; simpl; intros;
+    repeat (invert_exec; simpl in *; cleanup);
+    simpl; eauto; try solve [intuition].
+  -
+    eapply layer1_exec_finished_deterministic in H0; eauto; cleanup; eauto.
+    apply app_inv_head in H4; cleanup; eauto.
+  -
+    split_ors; cleanup.
+    exfalso; clear H2; eapply layer1_finished_not_crashed_oracle_app; eauto.
+
+    eapply layer1_exec_finished_deterministic in H0; eauto; cleanup; eauto.
+    apply app_inv_head in H4; cleanup; eauto.
     
-  - eapply exec_finished_deterministic in H0; eauto; cleanup.
-    eapply exec_finished_deterministic in H3; eauto; cleanup; eauto.
-  
-  - destruct H0; cleanup.
-    + exfalso; eapply exec_finished_oracle_app in H1; eauto; cleanup.  
-    + eapply exec_finished_deterministic in H0; eauto; cleanup.
-      apply app_inv_head in H4; cleanup; eauto.
+  -
+    split_ors; cleanup.
+    exfalso; clear H2; eapply layer1_finished_not_crashed_oracle_app; eauto.
 
-  - destruct H1; cleanup.
-    + exfalso; eapply exec_finished_oracle_app in H1; eauto; cleanup.  
-    + eapply exec_finished_deterministic in H0; eauto; cleanup.
-      apply app_inv_head in H4; cleanup; eauto.
+    eapply layer1_exec_finished_deterministic in H0; eauto; cleanup; eauto.
+    apply app_inv_head in H4; cleanup; eauto.
+  -
+    repeat split_ors; cleanup.
+    specialize IHp with (1:= H0)(2:= H1); cleanup; eauto.
 
-  - destruct H0; cleanup; destruct H1; cleanup.
-    + specialize IHp with (1:= H0)(2:=H1); cleanup; eauto.
-    + exfalso; eapply exec_finished_oracle_app in H1; eauto; cleanup.
-    + exfalso; eapply exec_finished_oracle_app in H1; eauto; cleanup.      
-    + eapply exec_finished_deterministic in H0; eauto; cleanup.
-      apply app_inv_head in H4; cleanup; eauto.
+    exfalso; clear H2; eapply layer1_finished_not_crashed_oracle_app; eauto.
+    
+    exfalso; clear H2; eapply layer1_finished_not_crashed_oracle_app; eauto.
 
+    eapply layer1_exec_finished_deterministic in H0; eauto; cleanup; eauto.
+    apply app_inv_head in H4; cleanup; eauto.
 Qed.
 
   Lemma oracle_ok_nonempty:
     forall T (p: prog T) s,
       ~oracle_ok p [] s.
   Proof.
-    unfold not, oracle_ok;
-    induction p; simpl; intros; try intuition congruence.
+    unfold not;
+    induction p; simpl; intros; try (split_ors; cleanup); try intuition congruence.
     cleanup.
     symmetry in H0; apply app_eq_nil in H0; cleanup; eauto.
   Qed.
@@ -128,12 +96,7 @@ Qed.
       oracle_ok (Bind (Bind p1 p2) p3) o sl ->
       oracle_ok (Bind p1 (fun x => (Bind (p2 x) p3))) o sl.      
   Proof.
-    intros;
-      unfold oracle_ok in *; intuition.
-    fold (@oracle_ok T) in *;
-      fold (@oracle_ok T') in *;
-      fold (@oracle_ok T'') in *.
-    cleanup.
+    intros; simpl in *; cleanup.
     exists x1, (x2++x0).
     split.
     rewrite app_assoc; eauto.
@@ -156,7 +119,7 @@ Qed.
   Proof.
     induction p1; simpl; intros;
     try solve [  pose proof H;
-      unfold oracle_ok in *; intuition;
+      simpl in *; intuition;
         invert_exec; simpl in *; cleanup;
       split_ors; cleanup; inversion H1; subst; eauto;
       specialize H3 with (1:= H); eauto].
@@ -170,20 +133,13 @@ Qed.
     specialize H with (1:=H3)(2:= H1)(3:= H5).
     destruct H; intuition eauto.
     
-    unfold oracle_ok in H5; cleanup;
-    fold (@oracle_ok T) in *;
-      fold (@oracle_ok T') in *;
-      fold (@oracle_ok T'0) in *.
-
-    unfold oracle_ok; cleanup;
-    fold (@oracle_ok T) in *;
-      fold (@oracle_ok T') in *;
-      fold (@oracle_ok T'0) in *.
+    simpl in *; cleanup.
+    
     do 2 eexists; intuition eauto.
-    eapply deterministic_prog in H0; eauto; cleanup; eauto.
-    eapply deterministic_prog in H0; eauto; cleanup.
+    eapply layer1_exec_deterministic in H0; eauto; cleanup; eauto.
+    eapply layer1_exec_deterministic in H0; eauto; cleanup.
   Qed.
-
+(*
   Lemma oracle_ok_finished_eq:
     forall T (p: prog T) o1 o2 o1' o2' s s' r,
       exec o1 s p (Finished s' r) ->
@@ -208,8 +164,9 @@ Qed.
       o2=[].
   Proof.
      induction p; simpl; intros;
-     try solve [ unfold oracle_ok in *; intuition;
-        invert_exec; simpl in *; cleanup; eauto].
+     try solve [ intuition; invert_exec; simpl in *; cleanup; eauto].
+     split_ors; cleanup; invert_exec; eauto.
+     
      invert_exec; split_ors; cleanup.
 
      -
@@ -235,28 +192,28 @@ Qed.
     eapply_fresh oracle_ok_exec_crashed_app_nil in H; eauto; cleanup.
     rewrite app_nil_r; eauto.
   Qed.
-
+*)
    Lemma exec_then_oracle_ok:
     forall T (p: prog T) o s r,
       exec o s p r ->
       oracle_ok p o s.
   Proof.
-    induction p; simpl; intros; try solve [unfold oracle_ok; invert_exec; cleanup; simpl; eauto].
+    induction p; simpl; intros; try solve [invert_exec; cleanup; simpl; eauto].
     invert_exec.
     - specialize IHp with (1:= H0).
       specialize H with (1:=H1).
       do 2 eexists; intuition; eauto;
-        eapply deterministic_prog in H0; eauto; cleanup; eauto.
+        eapply layer1_exec_deterministic in H0; eauto; cleanup; eauto.
     -
       split_ors; cleanup.
       specialize IHp with (1:= H0).
       do 2 eexists; intuition; eauto;
-        eapply deterministic_prog in H0; eauto; cleanup; eauto.
+        eapply layer1_exec_deterministic in H0; eauto; cleanup; eauto.
 
       specialize IHp with (1:= H0).
       specialize H with (1:=H1).
       do 2 eexists; intuition; eauto;
-        eapply deterministic_prog in H0; eauto; cleanup; eauto.
+        eapply layer1_exec_deterministic in H0; eauto; cleanup; eauto.
   Qed.
 
   Lemma finished_crash_not_in:
