src/Layer1/HoareLogic.v
@@ -3,6 +3,8 @@ Require Import Primitives Simulation Layer1.Definitions ProgAuto.
 Module Layer1 <: Layer.
   Definition oracle := oracle.
   Definition data := set value.
+  Definition aux_state := ((list key * encryptionmap) * hashmap)%type.
+  Definition state := (aux_state * disk data)%type.
   Definition prog := prog.
   Definition exec := exec.
   Definition oracle_ok := (fun T => @oracle_ok T).
@@ -15,10 +17,10 @@ Export Layer1HL.
 Arguments exec {T}.
 
 Theorem hoare_triple_equivalence :
-  forall T (p p': prog T) o d pre post crash ap ac,
-    hoare_triple pre p post crash ap ac o d ->
+  forall T (p p': prog T) o d a pre post crash ap ac,
+    hoare_triple pre p post crash ap ac o d a ->
     prog_equiv p p' ->
-    hoare_triple pre p' post crash ap ac o d.
+    hoare_triple pre p' post crash ap ac o d a.
 Proof.
   unfold hoare_triple; intros.
   edestruct H; eauto; cleanup.
@@ -32,7 +34,7 @@ Qed.
 
 Ltac monad_simpl_one :=
   match goal with
-  | [ |- hoare_triple _ (Bind (Bind _ _) _) _ _ ] =>
+  | [ |- hoare_triple _ (Bind (Bind _ _) _) _ _ _ _ _ _ _] =>
     eapply hoare_triple_equivalence;
     [ | apply bind_assoc ]
   end.
@@ -41,155 +43,174 @@ Ltac monad_simpl := repeat monad_simpl_one.
 
 
 Theorem bind_ok:
-  forall T T' (p1: prog T) (p2: T -> prog T') pre1 post1 crash1 pre2 post2 crash2 pre3 post3 crash3 o d,
+  forall T T' (p1: prog T) (p2: T -> prog T') pre1 post1 crash1 pre2 post2 crash2 pre3 post3 crash3 o d a,
   (forall o1,
    (exists o2, o = o1++o2) ->      
-   << o1, d >>
-   pre1
+   << o1, d, a >>
+   (pre1 a)
    p1
-  << r >>
-   (post1 r)
-   crash1) ->
-  ( pre3 =p=> pre1 ) ->
-  (forall F r,
-      (F * pre1)%pred d ->
-      post1 r =p=> pre2) ->
-  (forall F d2 r1 r2,
-      (F * pre1)%pred d ->
-      (F * post1 r1)%pred d2 ->
-      (F * pre2)%pred d2 ->
-      post2 r2 =p=> post3 r2) ->
-  (forall F,
-      (F * pre1)%pred d ->
-      crash1 =p=> crash3) ->
-  (forall F d2 r1,
-      (F * pre1)%pred d ->
-      (F * post1 r1)%pred d2 ->
-      (F * pre2)%pred d2 ->
-      crash2 =p=> crash3) ->
-  (forall F o2 d2 r,
-      (F * pre1)%pred d ->
-      (F * post1 r)%pred d2 ->
+  << r, ar >>
+   (post1 r ar)
+   (crash1 ar)) ->
+  ( pre3 a =p=> pre1 a) ->
+  (forall F r ar,
+      (F * pre1 a)%pred d ->
+      post1 r ar =p=> pre2 ar) ->
+  (forall F d2 r1 ar1 r2 ar2,
+      (F * pre1 a)%pred d ->
+      (F * post1 r1 ar1)%pred d2 ->
+      (F * pre2 ar1)%pred d2 ->
+      post2 r2 ar2 =p=> post3 r2 ar2) ->
+  (forall F ar,
+      (F * pre1 a)%pred d ->
+      crash1 ar =p=> crash3 ar) ->
+  (forall F d2 r1 ar1 ar2,
+      (F * pre1 a)%pred d ->
+      (F * post1 r1 ar1)%pred d2 ->
+      (F * pre2 ar1)%pred d2 ->
+      crash2 ar2 =p=> crash3 ar2) ->
+  (forall F o2 d2 r a2,
+      (F * pre1 a)%pred d ->
+      (F * post1 r a2)%pred d2 ->
       (exists o1, o = o1++o2) ->   
-      << o2, d2 >>
-         pre2
+      << o2, d2, a2 >>
+         (pre2 a2)
          (p2 r)
-       << r >>
-       (post2 r)
-       crash2) ->
-  << o, d >>
-     pre3
+       << r, ar >>
+       (post2 r ar)
+       (crash2 ar)) ->
+  << o, d, a >>
+     (pre3 a)
      (Bind p1 p2)
-  << r >>
-     (post3 r)
-     crash3.
+  << r, ar >>
+     (post3 r ar)
+     (crash3 ar).
 Proof.
   unfold hoare_triple, exec; intros.
   simpl in *; destruct_lifts; cleanup.
-  rewrite H0 in H6.
+  (* rewrite H0 in H6. *)
   edestruct H; eauto.
   pred_apply' H6; cancel; eauto.
+  eassign F; cancel; eauto.
   
   cleanup.
   split_ors; cleanup.
   - specialize H9 with (1:=H7).
     edestruct H5; eauto.
+    pred_apply; cancel; eauto.
     pred_apply' H12; norm.
     cancel.
-    erewrite H1; eauto; cancel.
+    eassign F; cancel.
+    eapply H1.
+    pred_apply; eassign F; cancel; eauto.
     intuition eauto.
+    destruct x2; simpl in *; eauto.
 
     cleanup.
+    destruct x2; simpl in *.
     split_ors; cleanup;
       eexists; split; intuition eauto.
 
     left; do 2 eexists; intuition eauto.
     pred_apply; cancel; eauto.
     eapply H2; eauto.
-    erewrite <- H1; eauto.
+    pred_apply; cancel; eauto.
+    pred_apply' H12; cancel; eauto.
+    eapply H1.
+    pred_apply; eassign F; cancel; eauto.
     
     right; eexists; intuition eauto.
     pred_apply; cancel; eauto.
     eapply H4; eauto.
-    erewrite <- H1; eauto.
+    pred_apply; cancel; eauto.
+    pred_apply' H12; cancel; eauto.
+    eapply H1.
+    pred_apply; eassign F; cancel; eauto.
+    
   - specialize H10 with (1:=H7); cleanup.
     rewrite app_nil_r.
     eexists; split; intuition eauto.
     right; eexists; intuition eauto.
     pred_apply' H12; cancel.
-    eauto.
+    eapply H3.
+    pred_apply; eassign F; cancel; eauto.
 Qed.
 
 Theorem bind_ok_aug:
-  forall T T' (p1: prog T) (p2: T -> prog T') pre1 post1 crash1 pre2 post2 crash2 pre3 post3 crash3 augpost augcrash o d,
+  forall T T' (p1: prog T) (p2: T -> prog T') pre1 post1 crash1 pre2 post2 crash2 pre3 post3 crash3 augpost augcrash o d a,
   (forall o1,
    (exists o2, o = o1++o2) ->
-   << o1, d >>
-   pre1
+   << o1, d, a >>
+   (pre1 a)
    p1
-  << r >>
-   (post1 r)
-   crash1) ->
-  ( pre3 =p=> pre1 ) ->
-  (forall F r,
-      (F * pre1)%pred d ->
-      post1 r =p=> pre2) ->
-  (forall F d2 r1 r2,
-      (F * pre1)%pred d ->
-      (F * post1 r1)%pred d2 ->
-      (F * pre2)%pred d2 ->
-      post2 r2 =p=> post3 r2) ->
-  (forall F,
-      (F * pre1)%pred d ->
-      crash1 =p=> crash3) ->
-  (forall F d2 r1,
-      (F * pre1)%pred d ->
-      (F * post1 r1)%pred d2 ->
-      (F * pre2)%pred d2 ->
-      crash2 =p=> crash3) ->
-  (forall o1 o2 F d1 r1,
-      (F * pre1)%pred d ->
-      exec o1 d p1 (Finished d1 r1) ->
-      (F * post1 r1)%pred d1 ->
+  << r, ar >>
+   (post1 r ar)
+   (crash1 ar)) ->
+  ( pre3 a =p=> pre1 a) ->
+  (forall F r ar,
+      (F * pre1 a)%pred d ->
+      post1 r ar =p=> pre2 ar) ->
+  (forall F d2 r1 ar1 r2 ar2,
+      (F * pre1 a )%pred d ->
+      (F * post1 r1 ar1)%pred d2 ->
+      (F * pre2 ar1)%pred d2 ->
+      post2 r2 ar2 =p=> post3 r2 ar2) ->
+  (forall F ar,
+      (F * pre1 a)%pred d ->
+      crash1 ar =p=> crash3 ar) ->
+  (forall F d2 r1 ar1 ar2,
+      (F * pre1 a)%pred d ->
+      (F * post1 r1 ar1)%pred d2 ->
+      (F * pre2 ar1)%pred d2 ->
+      crash2 ar2 =p=> crash3 ar2) ->
+  (forall o1 o2 F d' r1,
+      let a1 := fst d' in
+      let d1 := snd d' in
+      (F * pre1 a)%pred d ->
+      exec o1 (a, d) p1 (Finished d' r1) ->
+      (F * post1 r1 a1)%pred d1 ->
       (o = o1++o2) ->
-      << o2, d1 >>
-         pre2
+      << o2, d1, a1 >>
+         (pre2 a1)
          (p2 r1)
-       << r >>
-       (post2 r)
-       crash2
-       (augpost o d r)
-       (augcrash o d)
+       << r, ar >>
+       (post2 r ar)
+       (crash2 ar)
+       (augpost o a d r)
+       (augcrash o a d)
        ) ->
   (forall F o1 d',
-      (F * pre1)%pred d ->
-      exec o1 d p1 (Crashed d') ->
-      (F * crash1)%pred d' ->
+      (F * pre1 a)%pred d ->
+      exec o1 (a, d) p1 (Crashed d') ->
+      (F * crash1 (fst d'))%pred (snd d') ->
       (exists o2, o = o1++o2) ->
-      (F * augcrash o d)%pred d') ->
-  << o, d >>
-     pre3
+      (F * augcrash o a d)%pred (snd d')) ->
+  << o, d, a >>
+     (pre3 a)
      (Bind p1 p2)
-  << r >>
-     (post3 r)
-     crash3
-     (augpost o d r)
-     (augcrash o d)
+  << r, ar >>
+     (post3 r ar)
+     (crash3 ar)
+     (augpost o a d r)
+     (augcrash o a d)
      .
 Proof.
   unfold hoare_triple, exec; intros.
   simpl in *; destruct_lifts; cleanup.
-  rewrite H0 in H7.
+  (* rewrite H0 in H7. *)
   edestruct H; eauto.
   pred_apply' H7; cancel; eauto.
+  eassign F; cancel; eauto.  
   
   cleanup.
-  split_ors; cleanup.
+  split_ors; cleanup; destruct x2; simpl in *.
   - specialize H10 with (1:=H8).
     edestruct H5; eauto.
+    pred_apply; cancel; eauto.
     pred_apply' H13; norm.
-    cancel.
-    erewrite H1; eauto; cancel.
+    eassign F; cancel.
+    eapply H1.
+    pred_apply; eassign F; cancel; eauto.
     intuition eauto.
 
     cleanup.
@@ -198,19 +219,30 @@ Proof.
 
     left; do 2 eexists; intuition eauto.
     pred_apply' H16; cancel; eauto.
-    eapply H2; eauto.
-    erewrite <- H1; eauto.
+    eapply H2; eauto.    
+    pred_apply; cancel; eauto.
+    pred_apply' H13; norm. cancel.
+    eapply H1.
+    pred_apply; eassign F; cancel; eauto.
+    intuition.
     
     right; eexists; intuition eauto.
     pred_apply' H16; cancel; eauto.
     eapply H4; eauto.
-    erewrite <- H1; eauto.
+    pred_apply; cancel; eauto.
+    pred_apply' H13; norm. cancel.
+    eapply H1.
+    pred_apply; eassign F; cancel; eauto.
+    intuition.
+    
   - specialize H11 with (1:=H8); cleanup.
     rewrite app_nil_r in *.
     eexists; split; intuition eauto.
     right; eexists; intuition eauto.
     pred_apply' H13; cancel.
-    eauto.
+    eapply H3; eauto.    
+    pred_apply; eassign F; cancel; eauto.
     eapply H6; eauto.
+    pred_apply; cancel; eauto.
     exists nil; rewrite app_nil_r; eauto.
 Qed.
